proof/theories/Generated/Ruleset_Gen.v
@@ -1,20 +1,47 @@
 (* AUTO-GENERATED from ../../rulesets/ruleset.nft by nft2coq (extracted/nft_emit.ml). DO NOT EDIT.
-   This is the parser's output as Coq terms: the chains and the set/map
-   declarations their lookups read.  Properties proved about these terms
-   are properties of the parsed ruleset (and, via compile_table_correct, of
-   the installed bytecode). *)
+   This is the parser's SURFACE output as a Coq [sruleset]; the tables,
+   chains, hooks and set/map declarations the proofs reason about are the
+   VERIFIED lowering [Lower.lower_ruleset] applied to it (no hand-written
+   bytes here).  A refused construct fails [ruleset_lowers_ok] (fail-loud). *)
 
 From Stdlib Require Import List String ZArith.
 From Nft Require Import Bytes Verdict Packet Bytecode Syntax Semantics Nftval Elab.
+From Nft Require Import Surface.Ast Surface.Lower Gen_Support.
 Import ListNotations.
 Open Scope string_scope.
 
-Definition decls : set_decls :=
-  {| sd_sets := [("__set0", [(SEl [135]); (SEl [134]); (SEl [136])]);
-   ("__set3", [(SEl [0; 22]); (SEl [0; 80]); (SEl [1; 187])])];
-   sd_vmaps := [("__map1", [([0; 0; 0; 2], [0; 0; 0; 2], Accept); ([0; 0; 0; 4], [0; 0; 0; 4], Accept); ([0; 0; 0; 1], [0; 0; 0; 1], Drop)]);
-   ("__map2", [([8; 0], [8; 0], (Jump "inbound_ipv4")); ([134; 221], [134; 221], (Jump "inbound_ipv6"))])];
-   sd_maps := [] |}.
+Definition ruleset_surface : sruleset :=
+  [TopNop;
+
+   (TopTable {| st_family := "inet"; st_name := "firewall";
+      st_items := [(TChain {| sc_name := "inbound_ipv4";
+        sc_items := [] |});
+      (TChain {| sc_name := "inbound_ipv6";
+        sc_items := [(IRule [(CMatch {| sm_keys := [["icmpv6"; "type"]]; sm_rhs := {| sr_op := SOpImplicit; sr_neg := false; sr_payload := (SSEset [(SVSym "nd-neighbor-solicit"); (SVSym "nd-router-advert"); (SVSym "nd-neighbor-advert")]) |} |});
+           (CVerdict SVaccept)])] |});
+      (TChain {| sc_name := "inbound";
+        sc_items := [(ITypeHook "filter" "input" false 0);
+         (IPolicy SVdrop);
+         (IRule [(CVmap [["ct"; "state"]] [((SVSym "established"), SVaccept); ((SVSym "related"), SVaccept); ((SVSym "invalid"), SVdrop)])]);
+         (IRule [(CMatch {| sm_keys := [["iifname"]]; sm_rhs := {| sr_op := SOpImplicit; sr_neg := false; sr_payload := (SSEvalue (SVSym "lo")) |} |});
+           (CVerdict SVaccept)]);
+         (IRule [(CVmap [["meta"; "protocol"]] [((SVSym "ip"), (SVjump "inbound_ipv4")); ((SVSym "ip6"), (SVjump "inbound_ipv6"))])]);
+         (IRule [(CMatch {| sm_keys := [["tcp"; "dport"]]; sm_rhs := {| sr_op := SOpImplicit; sr_neg := false; sr_payload := (SSEset [(SVNum 22); (SVNum 80); (SVNum 443)]) |} |});
+           (CVerdict SVaccept)])] |});
+      (TChain {| sc_name := "forward";
+        sc_items := [(ITypeHook "filter" "forward" false 0);
+         (IPolicy SVdrop)] |})] |})].
+
+Definition ifindex_pins (s : string) : option nat :=
+  if String.eqb s "lo" then Some 1%nat else None.
+
+Example ruleset_lowers_ok : lower_ok ifindex_pins ruleset_surface = true.
+Proof. vm_compute. reflexivity. Qed.
+
+Definition ruleset_lowered : lowered_ruleset :=
+  Eval vm_compute in lower_or_empty ifindex_pins ruleset_surface.
+
+Definition decls : set_decls := Eval vm_compute in lr_set_decls ruleset_lowered.
 
 Definition base_env : env :=
   {| e_set := fun _ => []; e_vmap := fun _ => []; e_map := fun _ => [];
@@ -28,42 +55,20 @@ Definition gen_env : env := env_with_sets base_env decls.
 (* ===== table inet firewall ===== *)
 
 Definition firewall_inbound_ipv4 : chain :=
-  {| c_policy := Continue;
-   c_rules := [] |}.
+  Eval vm_compute in lr_chain_of ruleset_lowered "firewall" "inbound_ipv4".
 
 Definition firewall_inbound_ipv6 : chain :=
-  {| c_policy := Continue;
-   c_rules := [{| r_body := [(BDep (elab_m (TMEq FMetaNfproto (VInteger 1 10))));
-             (BDep (elab_m (TMEq FMetaL4proto (VInteger 1 58))));
-             (BMatch (MConcatSet [FIcmpType] false "__set0"))];
-     r_outcome := OVerdict Accept; r_after := [] |}] |}.
+  Eval vm_compute in lr_chain_of ruleset_lowered "firewall" "inbound_ipv6".
 
 Definition firewall_inbound : chain :=
-  {| c_policy := Drop;
-   c_rules := [{| r_body := [];
-     r_outcome := OVmap {| vm_fields := []; vm_keyf := (Some (FCtState, [])); vm_name := "__map1" |}; r_after := [] |};
-
-   {| r_body := [(BMatch (elab_m (TMEq FMetaIifname (ifname "lo"))))];
-     r_outcome := OVerdict Accept; r_after := [] |};
-
-   {| r_body := [];
-     r_outcome := OVmap {| vm_fields := []; vm_keyf := (Some (FMetaProtocol, [])); vm_name := "__map2" |}; r_after := [] |};
-
-   {| r_body := [(BDep (elab_m (TMEq FMetaL4proto (VInteger 1 6))));
-             (BMatch (MConcatSet [FThDport] false "__set3"))];
-     r_outcome := OVerdict Accept; r_after := [] |}] |}.
+  Eval vm_compute in lr_chain_of ruleset_lowered "firewall" "inbound".
 
 Definition firewall_forward : chain :=
-  {| c_policy := Drop;
-   c_rules := [] |}.
+  Eval vm_compute in lr_chain_of ruleset_lowered "firewall" "forward".
 
 Definition firewall_chains : list (string * chain) :=
-  [("inbound_ipv4", firewall_inbound_ipv4);
-   ("inbound_ipv6", firewall_inbound_ipv6);
-   ("inbound", firewall_inbound);
-   ("forward", firewall_forward)].
+  Eval vm_compute in lr_chains_of ruleset_lowered "firewall".
 
 Definition firewall_hooks : list hooked_chain :=
-  [{| hc_hook := Hinput; hc_prio := (0)%Z; hc_env := firewall_chains; hc_base := firewall_inbound |};
-   {| hc_hook := Hforward; hc_prio := (0)%Z; hc_env := firewall_chains; hc_base := firewall_forward |}].
+  Eval vm_compute in lr_hooks_of ruleset_lowered "firewall".
 
